src/Invariant.v
@@ -1,0 +1,84 @@
+Require Import Bool List String Peano_dec.
+Require Import Common FMap ListSupport Syntax Semantics StepDet SemFacts.
+Require Import Serial.
+
+Set Implicit Arguments.
+
+Section Invariant.
+  Variables (SysI StateI LabelI: Type).
+  Context `{IsSystem SysI StateI} `{HasLabel LabelI}.
+
+  Variable (impl: SysI).
+
+  Variables (stepI: Step SysI StateI LabelI)
+            (ginv: StateI -> Prop).
+
+  Definition Invariant := StateI -> Prop.
+
+  Definition InvInit := ginv (initsOf impl).
+
+  Definition InvStep :=
+    forall ist1,
+      ginv ist1 ->
+      forall lbl ist2,
+        stepI impl ist1 lbl ist2 ->
+        ginv ist2.
+
+  Definition InvSteps :=
+    forall ist1,
+      ginv ist1 ->
+      forall lbl ist2,
+        steps stepI impl ist1 lbl ist2 ->
+        ginv ist2.
+
+  Hypotheses (Hinvi: InvInit)
+             (Hinvs: InvStep).
+
+  Lemma inv_steps':
+    forall ist1,
+      ginv ist1 ->
+      forall ihst ist2,
+        steps stepI impl ist1 ihst ist2 ->
+        ginv ist2.
+  Proof.
+    induction 2; simpl; intros; eauto.
+  Qed.
+
+  Lemma inv_steps: InvSteps.
+  Proof.
+    unfold InvSteps; intros.
+    eapply inv_steps'; eauto.
+  Qed.
+  
+End Invariant.
+
+Section Operations.
+  Context {StateT: Type}.
+
+  Definition invAnd (inv1 inv2: Invariant StateT) :=
+    fun tst => inv1 tst /\ inv2 tst.
+
+  Definition invImp (inv1 inv2: Invariant StateT) :=
+    forall tst, inv1 tst -> inv2 tst.
+
+  Lemma tinv_proj1: forall inv1 inv2, invImp (invAnd inv1 inv2) inv1.
+  Proof. firstorder. Qed.
+  Lemma tinv_proj2: forall inv1 inv2, invImp (invAnd inv1 inv2) inv2.
+  Proof. firstorder. Qed.
+
+  Lemma inv_split:
+    forall (inv1 inv2: Invariant StateT) st,
+      inv1 st ->
+      inv2 st ->
+      (invAnd inv1 inv2) st.
+  Proof.
+    unfold invAnd; intros; dest; split; eauto.
+  Qed.
+
+End Operations.
+
+Ltac split_inv := apply inv_split.
+
+Infix "/\i" := invAnd (at level 80).
+Infix "->i" := invImp (at level 99).
+
